workspace/src/login/DY.Login.Proof.fst
@@ -124,8 +124,8 @@ let api_request_proof tr comm_keys_ids client sid =
       let ((), tr_event) = trigger_event client (ClientAuthenticatesToServer client server) tr_gd1 in
       assert(trace_invariant tr_event);
       let (url, http_req) = build_login_request client password in
-      let (opt_server, tr_gd2) = guard_tr (server = http_config_login.domain_to_principal url.domain) tr_event in
-      match opt_server with
+      let (opt_gd1, tr_gd2) = guard_tr (server = http_config_login.domain_to_principal url.domain) tr_event in
+      match opt_gd1 with
       | None -> ()
       | Some _ ->
         assert(tr_event == tr_gd2);
@@ -145,12 +145,20 @@ let api_request_proof tr comm_keys_ids client sid =
 
 (*** API Server ***)
 
+#restart-solver
 #push-options "--fuel 6 --z3rlimit 40"
 val build_login_response_proof:
   tr:trace -> hmeta_data:http_meta_data web_types kv_types ->
+  client:principal -> cookie:cookie_t ->
   Lemma
+  (requires
+    event_triggered tr hmeta_data.server (ServerAuthenticatedClient client hmeta_data.server cookie) /\
+    is_secret (get_response_label tr hmeta_data) tr cookie.value /\
+    cookie.secure == true /\
+    Some? (get_set_cookie_header "accessToken" [SetCookie cookie <: header_t kv_types])
+  )
   (ensures (
-    let http_res = build_login_response () in
+    let http_res = build_login_response client cookie in
     let http_req = Request?.http_req hmeta_data.request in
     is_well_formed
       (http_response_t web_types kv_types)
@@ -163,40 +171,49 @@ val build_login_response_proof:
       tr hmeta_data.client hmeta_data.server http_req http_res
       (get_response_label tr hmeta_data)
   ))
-let build_login_response_proof tr hmeta_data =
+let build_login_response_proof tr hmeta_data client cookie =
   reveal_opaque (`%build_login_response) build_login_response;
   let headers:list (header_t kv_types) = [
-    ContentType "application/json"
+    ContentType "application/json";
+    SetCookie cookie
   ] in
   let body = JSON [
     {key = "id"; value = VI 1};
-    {key = "username"; value = VS "emilys"};
+    {key = "username"; value = VS client};
     {key = "email"; value = VS "emily.johnson@x.dummyjson.com"};
     {key = "firstName"; value = VS "Emily"};
     {key = "lastName"; value = VS "Johnson"}
   ] in
   let http_res = mk_http_response 200 headers body in
   let http_req = Request?.http_req hmeta_data.request in
+  
+  // Proving is_well_formed
   let lab = get_response_label tr hmeta_data in
   assert (for_allP (is_knowable_by_web_kv lab tr) (JSON?._0 body));
   web_types_serialization_lemma tr body lab;
   assert (for_allP (is_knowable_by_header lab tr) headers);
   mk_http_response_knowable
     tr hmeta_data.server hmeta_data 200 headers body;
+  assert(is_well_formed
+      (http_response_t web_types kv_types)
+      (is_knowable_by lab tr)
+      http_res);
+  
+  // Proving body_preds_web_types.http_body_response_pred
   web_types_response_key_pred_implies_global_pred
-    tr "id" (wt_send_request_pred_key_true "id")
+    tr "id" (wt_send_response_pred_key_true "id")
     hmeta_data http_req http_res;
   web_types_response_key_pred_implies_global_pred
-    tr "username" (wt_send_request_pred_key_true "username")
+    tr "username" (wt_send_response_pred_key_username)
     hmeta_data http_req http_res;
   web_types_response_key_pred_implies_global_pred
-    tr "email" (wt_send_request_pred_key_true "email")
+    tr "email" (wt_send_response_pred_key_true "email")
     hmeta_data http_req http_res;
   web_types_response_key_pred_implies_global_pred
-    tr "firstName" (wt_send_request_pred_key_true "firstName")
+    tr "firstName" (wt_send_response_pred_key_true "firstName")
     hmeta_data http_req http_res;
   web_types_response_key_pred_implies_global_pred
-    tr "lastName" (wt_send_request_pred_key_true "lastName")
+    tr "lastName" (wt_send_response_pred_key_true "lastName")
     hmeta_data http_req http_res;
   assert (
     for_allP_web_types
@@ -205,15 +222,32 @@ let build_login_response_proof tr hmeta_data =
       body
   );
   forall_web_types_response_preds_implies_comm_reqres_preds_lemma
-    tr hmeta_data 200 headers body
+    tr hmeta_data 200 headers body;
+  assert(body_preds_web_types.http_body_response_pred
+      tr hmeta_data.client hmeta_data.server http_req http_res
+      lab);
+  
+  // Proving http_response_properties
+  assert(for_allP (http_response_header_properties tr hmeta_data.client hmeta_data.server http_req http_res lab) headers) by (
+    let open FStar.Tactics in
+    norm [delta_only [`%for_allP; `%http_response_header_properties]; iota; zeta];
+    ()
+  );
+  mk_http_response_headers_extractable 200 headers body;
+  assert(for_allP (http_response_header_properties tr hmeta_data.client hmeta_data.server http_req http_res lab) http_res.headers);
+  assert(http_response_properties
+      tr hmeta_data.client hmeta_data.server http_req http_res
+      lab);
+  ()
 #pop-options
 
 #push-options "--z3rlimit 20"
-val helper_lemma_event_invariant:
+val helper_lemma_event_invariant_server_authenticated_client:
   tr:trace -> client:principal -> server:principal ->
   http_req:http_request_t web_types kv_types ->
   hmeta_data:http_meta_data web_types kv_types ->
   password:bytes ->
+  cookie:cookie_t ->
   Lemma
   (requires
     trace_invariant tr /\
@@ -224,34 +258,37 @@ val helper_lemma_event_invariant:
     get_bytes_from_json_encoded "password" http_req.body == Some password /\
     get_principal_from_json_encoded "username" http_req.body == Some client /\
     is_secret (comm_label client server) tr password /\
-    is_server_request http_req
+    is_server_request http_req /\
+    is_secret (get_response_label tr hmeta_data) tr cookie.value
   )
   (ensures (
-    event_predicate_login tr server (ServerAuthenticatedClient client server)
+    event_predicate_login tr server (ServerAuthenticatedClient client server cookie)
   ))
-let helper_lemma_event_invariant tr client server http_req hmeta_data password =
+let helper_lemma_event_invariant_server_authenticated_client tr client server http_req hmeta_data password cookie =
   eliminate (exists client. event_triggered tr client (CommClientSendRequest Unauthenticated client server hmeta_data.request hmeta_data.key <: communication_reqres_event (http_t web_types kv_types))) \/
     (is_publishable tr hmeta_data.key /\ is_well_formed (http_t web_types kv_types) (is_publishable tr) hmeta_data.request)
-  returns event_triggered tr client (ClientAuthenticatesToServer client server) \/
+  returns (event_triggered tr client (ClientAuthenticatesToServer client server) /\
+        is_secret (comm_label client server) tr cookie.value) \/
     is_corrupt tr (principal_label client) \/ is_corrupt tr (principal_label server)
   with _. (
     eliminate exists client. event_triggered tr client (CommClientSendRequest Unauthenticated client server hmeta_data.request hmeta_data.key <: communication_reqres_event (http_t web_types kv_types))
-    returns event_triggered tr client (ClientAuthenticatesToServer client server) \/
+    returns (event_triggered tr client (ClientAuthenticatesToServer client server) /\
+        is_secret (comm_label client server) tr cookie.value) \/
       is_corrupt tr (principal_label client) \/ is_corrupt tr (principal_label server)
     with _. (
       web_types_request_predicate tr "username" wt_send_request_pred_key_username hmeta_data client;
+      get_response_label_eq_key_label tr hmeta_data;
       ()
     )
   )
   and _. (
     assert(is_well_formed web_types (is_publishable tr) http_req.body);
     get_bytes_from_json_encoded_knowable tr public "password" http_req.body;
-    assert(is_publishable tr password);
     ()
   )
 #pop-options
 
-#push-options "--ifuel 1 --z3rlimit 40"
+#push-options "--ifuel 1 --z3rlimit 100"
 val api_server_proof:
   tr:trace -> comm_keys_ids:communication_keys_sess_ids ->
   server:principal -> sid:state_id -> msg_id:timestamp ->
@@ -266,42 +303,112 @@ val api_server_proof:
 let api_server_proof tr comm_keys_ids server sid msg_id =
   reveal_opaque (`%api_server) (api_server comm_keys_ids server sid msg_id);
   let (_, tr_out) = api_server comm_keys_ids server sid msg_id tr in
+  
   let (opt_state, tr_get) = get_state #state_t server sid tr in
+  assert(trace_invariant tr_get);
   match opt_state with
   | None -> ()
   | Some (SendRequest _) -> ()
   | Some (InitialState client state_server password) ->
-    let (opt_server, tr_gd1) = guard_tr (server = state_server) tr_get in
-    match opt_server with
+    let (opt_gd1, tr_gd1) = guard_tr (server = state_server) tr_get in
+    assert(trace_invariant tr_gd1);
+    match opt_gd1 with
     | None -> ()
     | Some _ ->
       receive_https_request_proof #protocol_invariants_login #web_types #kv_types tr_gd1 comm_keys_ids server msg_id;
       let (opt_request, tr_received) = receive_https_request comm_keys_ids server msg_id tr_gd1 in
+      assert(trace_invariant tr_received);
       match opt_request with
       | None -> ()
       | Some (http_req, hmeta_data) ->
         let (opt_user_agent, tr_gd2) = guard_tr (get_user_agent_header http_req.headers = Some Server) tr_received in
+        assert(trace_invariant tr_gd2);
         match opt_user_agent with
         | None -> ()
         | Some _ ->
           let (credentials_match, tr_gd3) = guard_tr (login_request_credentials_match client password http_req) tr_gd2 in
+          assert(trace_invariant tr_gd3);
           match credentials_match with
           | None -> ()
           | Some _ ->
-            let ((), tr_event) = trigger_event server (ServerAuthenticatedClient client server) tr_gd3 in
-            helper_lemma_event_invariant tr_gd3 client server http_req hmeta_data password;
-            assert(trace_invariant tr_event);
-            
-            let (_, tr_snd) = send_https_response server hmeta_data (build_login_response ()) tr_event in
-            build_login_response_proof tr_event hmeta_data;
-            send_https_response_proof tr_event server hmeta_data (build_login_response ());
-            assert(trace_invariant tr_snd);
-            assert (tr_snd == tr_out);
-            ()
+            let real_cookie = serialize usage_rand_string {rand = "secret"} in
+            let (opt_cookie, tr_nonce) = mk_comm_layer_response_nonce hmeta_data (AeadKey "" real_cookie) tr_gd3 in
+            assert(trace_invariant tr_nonce);
+            match opt_cookie with
+            | None -> ()
+            | Some cookie_value ->
+              let cookie = {
+                  name = "accessToken";
+                  value = cookie_value;
+                  http_only = true;
+                  secure = true;
+                } in
+              let ((), tr_event) = trigger_event server (ServerAuthenticatedClient client server cookie) tr_nonce in
+              helper_lemma_event_invariant_server_authenticated_client tr_nonce client server http_req hmeta_data password cookie;
+              assert(trace_invariant tr_event);
+              
+              let http_resp = build_login_response client cookie in
+              let (_, tr_snd) = send_https_response server hmeta_data http_resp tr_event in
+              
+              assert_norm(Some? (get_set_cookie_header "accessToken" [SetCookie cookie <: header_t kv_types]));
+              build_login_response_proof tr_event hmeta_data client cookie;
+              send_https_response_proof tr_event server hmeta_data http_resp;
+              assert(trace_invariant tr_snd);
+              assert (tr_snd == tr_out);
+              ()
 #pop-options
 
 
 (*** API Response ***)
+
+#restart-solver
+#push-options "--z3rlimit 20"
+val helper_lemma_event_invariant_client_received_cookie:
+  tr:trace -> client:principal -> hmeta_data:http_meta_data web_types kv_types -> http_res:http_response_t web_types kv_types -> cookie:cookie_t ->
+  Lemma
+  (requires
+    trace_invariant tr /\
+    get_set_cookie_header "accessToken" http_res.headers == Some cookie /\
+    get_string_from_json_encoded "username" http_res.body == Some client /\
+    is_server_request (Request?.http_req hmeta_data.request) /\
+    cookie.secure == true /\
+    event_triggered tr client (CommClientReceiveResponse client (Response http_res) hmeta_data <: communication_reqres_event (http_t web_types kv_types)) /\
+    event_triggered tr client (CommClientSendRequest (request_authenticated hmeta_data) client hmeta_data.server hmeta_data.request hmeta_data.key <: communication_reqres_event (http_t web_types kv_types))
+  )
+  (ensures (
+    event_predicate_login tr client (ClientReceivedCookie client hmeta_data.server cookie)
+  ))
+let helper_lemma_event_invariant_client_received_cookie tr client hmeta_data http_res cookie =
+  response_message_properties tr client (Response http_res) hmeta_data;
+  eliminate event_triggered tr hmeta_data.server (CommServerSendResponse hmeta_data.client hmeta_data.server hmeta_data.request (Response http_res) hmeta_data.key <: communication_reqres_event (http_t web_types kv_types)) \/
+    (is_corrupt tr (principal_label client) \/ is_corrupt tr (principal_label hmeta_data.server))
+  returns (event_triggered tr hmeta_data.server (ServerAuthenticatedClient client hmeta_data.server cookie) /\
+        is_secret (comm_label client hmeta_data.server) tr cookie.value) \/
+       is_corrupt tr (principal_label client) \/ is_corrupt tr (principal_label hmeta_data.server)
+  with _. (
+    let http_req = Request?.http_req hmeta_data.request in
+    comm_server_send_response_implies_set_cookie_properties tr client hmeta_data http_res "accessToken" cookie;
+    send_request_event_properties tr client hmeta_data;
+    web_types_response_predicate tr "username" wt_send_response_pred_key_username hmeta_data client http_res;
+    ()
+  )
+  and _. ()
+#pop-options
+
+#push-options "--ifuel 1 --z3rlimit 40"
+val process_login_response_proof:
+  client:principal -> http_res:http_response_t web_types kv_types -> 
+  Lemma
+  (ensures (
+    let opt_cookie = process_login_response client http_res in
+    match opt_cookie with
+    | Some cookie -> get_set_cookie_header "accessToken" http_res.headers == Some cookie /\
+      get_string_from_json_encoded "username" http_res.body == Some client /\
+      cookie.secure == true
+    | None -> True
+  ))
+let process_login_response_proof client http_res = ()
+#pop-options
 
 #push-options "--ifuel 1 --z3rlimit 20"
 val api_response_proof:
@@ -318,9 +425,31 @@ let api_response_proof tr client sid msg_id =
   reveal_opaque (`%api_response) (api_response client sid msg_id);
   let (_, tr_out) = api_response client sid msg_id tr in
 
-  match get_state #state_t client sid tr with
-  | (Some (SendRequest hmeta_data), _) ->
+  let (opt_state, tr_get) = get_state #state_t client sid tr in
+  assert(trace_invariant tr_get);
+  match opt_state with
+  | None -> ()
+  | Some (InitialState _ _ _) -> ()
+  | Some (SendRequest hmeta_data) ->
+    let (opt_response, tr_received) = receive_https_response hmeta_data client msg_id tr_get in
     receive_https_response_proof tr hmeta_data client msg_id;
-    assert (trace_invariant tr_out)
-  | _ -> ()
+    assert (trace_invariant tr_received);
+    match opt_response with
+    | None -> ()
+    | Some http_res ->
+      let (opt_cookie, tr_cookie) = return (process_login_response client http_res) tr_received in
+      process_login_response_proof client http_res;
+      assert (trace_invariant tr_cookie);
+      match opt_cookie with
+      | None -> ()
+      | Some cookie ->
+        let (opt_gd, tr_gd) = guard_tr (cookie.secure) tr_cookie in
+        match opt_gd with
+        | None -> ()
+        | Some _ ->
+          let ((), tr_event) = trigger_event client (ClientReceivedCookie client (hmeta_data.server) cookie) tr_gd in
+          helper_lemma_event_invariant_client_received_cookie tr_gd client hmeta_data http_res cookie;
+          assert (trace_invariant tr_event);
+          assert (tr_event == tr_out);
+          ()
 #pop-options
