workspace/src/login/DY.Login.Protocol.fst
@@ -35,7 +35,8 @@ instance local_state_state_t: local_state state_t = {
 [@@with_bytes bytes]
 type event_t =
   | ClientAuthenticatesToServer: client:principal -> server:principal -> event_t
-  | ServerAuthenticatedClient: client:principal -> server:principal -> event_t
+  | ServerAuthenticatedClient: client:principal -> server:principal -> cookie:cookie_t -> event_t
+  | ClientReceivedCookie: client:principal -> server:principal -> cookie:cookie_t -> event_t
 
 %splice [ps_event_t] (gen_parser (`event_t))
 %splice [ps_event_t_is_well_formed] (gen_is_well_formed_lemma (`event_t))
@@ -44,6 +45,7 @@ instance event_login: event event_t = {
   tag = "LoginAPI.Event";
   format = mk_parseable_serializeable ps_event_t;
 }
+
 
 (*** HTTP Library Initialization ***)
 
@@ -97,17 +99,6 @@ let api_request comm_keys_ids client sid =
   set_state client sid (SendRequest hmeta_data);*
   return (Some (sid, msg_id))
 
-val build_login_response: unit -> http_response_t web_types kv_types
-let build_login_response () =
-  let headers:list (header_t kv_types) = [ContentType "application/json"] in
-  let body = JSON [{
-    key = "id"; value = VI 1 };
-    {key = "username"; value = VS "emilys" };
-    {key =  "email"; value = VS "emily.johnson@x.dummyjson.com"};
-    {key = "firstName"; value = VS "Emily"};
-    {key = "lastName"; value = VS "Johnson"}] in
-  mk_http_response 200 headers body
-
 val login_request_credentials_match:
   principal -> bytes -> http_request_t web_types kv_types -> bool
 let login_request_credentials_match client password http_req =
@@ -115,6 +106,20 @@ let login_request_credentials_match client password http_req =
         get_bytes_from_json_encoded "password" http_req.body with
   | Some client', Some password' -> client = client' && password = password'
   | _ -> false
+
+val build_login_response: principal -> cookie_t -> http_response_t web_types kv_types
+let build_login_response client cookie =
+  let headers:list (header_t kv_types) = [
+    ContentType "application/json";
+    SetCookie cookie
+  ] in
+  let body = JSON [{
+    key = "id"; value = VI 1 };
+    {key = "username"; value = VS client};
+    {key =  "email"; value = VS "emily.johnson@x.dummyjson.com"};
+    {key = "firstName"; value = VS "Emily"};
+    {key = "lastName"; value = VS "Johnson"}] in
+  mk_http_response 200 headers body
 
 val api_server: communication_keys_sess_ids -> principal -> state_id -> timestamp -> traceful (option timestamp)
 let api_server comm_keys_ids server sid msg_id =
@@ -127,25 +132,39 @@ let api_server comm_keys_ids server sid msg_id =
   guard_tr (get_user_agent_header http_req.headers = Some Server);*?
   guard_tr (login_request_credentials_match client password http_req);*?
 
-  trigger_event server (ServerAuthenticatedClient client server);*
+  let real_cookie = serialize usage_rand_string {rand = "secret"} in
+  let*? cookie_value = mk_comm_layer_response_nonce hmeta_data (AeadKey "" real_cookie) in
+  let cookie = {
+      name = "accessToken";
+      value = cookie_value;
+      http_only = true;
+      secure = true;
+    } in
 
-  let*? msg_id_out = send_https_response server hmeta_data (build_login_response ()) in
+  trigger_event server (ServerAuthenticatedClient client server cookie);*
+
+  let http_resp = build_login_response client cookie in
+  let*? msg_id_out = send_https_response server hmeta_data http_resp in
   return (Some msg_id_out)
 
 val process_login_response:
-  http_response_t web_types kv_types -> option unit
-let process_login_response http_res =
+  client:principal -> http_response_t web_types kv_types -> option cookie_t
+let process_login_response client http_res =
   let? id = get_int_from_json_encoded "id" http_res.body in
   let _ = IO.debug_print_string (Printf.sprintf "\nReceived id: %d\n" id) in
   let? username = get_string_from_json_encoded "username" http_res.body in
   let _ = IO.debug_print_string (Printf.sprintf "Received username: %s\n" username) in
+  guard (username = client);?
   let? email = get_string_from_json_encoded "email" http_res.body in
   let _ = IO.debug_print_string (Printf.sprintf "Received email: %s\n" email) in
   let? firstName = get_string_from_json_encoded "firstName" http_res.body in
   let _ = IO.debug_print_string (Printf.sprintf "Received firstName: %s\n" firstName) in
   let? lastName = get_string_from_json_encoded "lastName" http_res.body in
   let _ = IO.debug_print_string (Printf.sprintf "Received lastName: %s\n\n" lastName) in
-  Some ()
+  let? cookie = get_set_cookie_header "accessToken" http_res.headers in
+  guard (cookie.secure);?
+  let _ = IO.debug_print_string (Printf.sprintf "Received cookie: %s\n" (bytes_to_string cookie.value)) in
+  Some cookie
 
 val api_response: principal -> state_id -> timestamp -> traceful (option unit)
 let api_response client sid msg_id =
@@ -153,4 +172,7 @@ let api_response client sid msg_id =
   guard_tr (SendRequest? st);*?
   let SendRequest hmeta_data = st in
   let*? http_res = receive_https_response hmeta_data client msg_id in
-  return (process_login_response http_res)
+  let*? cookie = return (process_login_response client http_res) in
+  guard_tr (cookie.secure);*?
+  trigger_event client (ClientReceivedCookie client hmeta_data.server cookie);*
+  return (Some ())
