workspace/src/login/DY.Login.SecurityProperties.fst
@@ -15,17 +15,30 @@ open DY.Login.Invariants
 #set-options "--fuel 0 --ifuel 0 --z3cliopt 'smt.qi.eager_threshold=100'"
 
 val user_authentication:
-  tr:trace -> client:principal -> server:principal -> 
+  tr:trace -> client:principal -> server:principal -> cookie:cookie_t ->
   Lemma
   (requires
     trace_invariant tr /\
-    event_triggered tr server (ServerAuthenticatedClient client server)
+    event_triggered tr server (ServerAuthenticatedClient client server cookie)
   )
   (ensures (
     event_triggered tr client (ClientAuthenticatesToServer client server) \/
     is_corrupt tr (principal_label client) \/ is_corrupt tr (principal_label server)
   ))
-let user_authentication tr client server = ()
+let user_authentication tr client server cookie = ()
+
+val server_authentication:
+  tr:trace -> client:principal -> server:principal -> cookie:cookie_t ->
+  Lemma
+  (requires
+    trace_invariant tr /\
+    event_triggered tr client (ClientReceivedCookie client server cookie)
+  )
+  (ensures (
+    event_triggered tr server (ServerAuthenticatedClient client server cookie) \/
+    is_corrupt tr (principal_label client) \/ is_corrupt tr (principal_label server)
+  ))
+let server_authentication tr client server cookie = ()
 
 val password_secrecy:
   tr:trace -> client:principal -> server:principal -> password:bytes ->
@@ -42,3 +55,19 @@ val password_secrecy:
   )
 let password_secrecy tr client server password =
   attacker_only_knows_publishable_values tr password
+
+val cookie_secrecy:
+  tr:trace -> client:principal -> server:principal -> cookie:cookie_t ->
+  Lemma
+  (requires
+    trace_invariant tr /\
+    attacker_knows tr cookie.value /\ (
+      event_triggered tr server (ServerAuthenticatedClient client server cookie) \/
+      event_triggered tr client (ClientReceivedCookie client server cookie)
+    )
+  )
+  (ensures
+    is_corrupt tr (principal_label client) \/ is_corrupt tr (principal_label server)
+  )
+let cookie_secrecy tr client server cookie =
+  attacker_only_knows_publishable_values tr cookie.value
